Orders.v
@@ -1,0 +1,409 @@
+Require Import List OrderedType OrderedTypeAlt OrderedTypeEx.
+Require Import GallStar.Tactics.
+Import ListNotations.
+
+Module Type UsualComparableType.
+
+  Parameter t : Type.
+
+  Parameter compare : t -> t -> comparison.
+
+  Parameter compare_eq :
+    forall x y : t,
+      compare x y = Eq <-> x = y. 
+
+  Parameter compare_trans :
+    forall (c : comparison) (x y z : t),
+      compare    x y = c
+      -> compare y z = c
+      -> compare x z = c.
+
+End UsualComparableType.
+
+Module UOT_from_UCT (C : UsualComparableType) <: UsualOrderedType.
+
+  Definition t := C.t.
+  
+  Definition eq       := @eq t.
+  Definition eq_refl  := @eq_refl t.
+  Definition eq_sym   := @eq_sym t.
+  Definition eq_trans := @eq_trans t.
+
+  Definition lt (x y : t) : Prop :=
+    match C.compare x y with
+    | Lt => True
+    | _  => False
+    end.
+
+  Lemma lt_trans :
+    forall x y z, lt x y -> lt y z -> lt x z.
+  Proof.
+    unfold lt; intros x y z hlt hlt'.
+    destruct (C.compare x y) eqn:hc  ;
+      destruct (C.compare y z) eqn:hc' ;
+      destruct (C.compare x z) eqn:hc''; auto.
+    - eapply C.compare_trans in hc'; eauto; tc.
+    - eapply C.compare_trans in hc'; eauto; tc.
+  Qed.
+  
+  Lemma lt_not_eq :
+    forall x y, lt x y -> ~ x = y.
+  Proof.
+    unfold lt; intros x y hl heq.
+    apply C.compare_eq in heq.
+    rewrite heq in hl; inv hl.
+  Qed.
+
+  Lemma compare_refl :
+    forall x, C.compare x x = Eq.
+  Proof.
+    intros x; apply C.compare_eq; auto.
+  Qed.
+  
+  Lemma compare_sym :
+    forall x y, C.compare x y = CompOpp (C.compare y x).
+  Proof.
+    intros x y; destruct (C.compare x y) eqn:hc.
+    - apply C.compare_eq in hc; subst.
+      rewrite compare_refl; auto.
+    - destruct (C.compare y x) eqn:hc'; auto.
+      + exfalso; apply C.compare_eq in hc'; subst.
+        rewrite compare_refl in hc; tc.
+      + exfalso; eapply C.compare_trans in hc'; eauto.
+        rewrite compare_refl in hc'; tc.
+    - destruct (C.compare y x) eqn:hc'; auto.
+      + exfalso; apply C.compare_eq in hc'; subst.
+        rewrite compare_refl in hc; tc.
+      + exfalso; eapply C.compare_trans in hc'; eauto.
+        rewrite compare_refl in hc'; tc.
+  Qed.
+
+  Definition compare :
+    forall x y,
+      Compare lt eq x y.
+  Proof.
+    intros x y; destruct (C.compare x y) eqn:hc.
+    - apply EQ; apply C.compare_eq; auto.
+    - apply LT; unfold lt; rewrite hc; auto.
+    - apply GT; unfold lt; rewrite compare_sym in hc.
+      destruct (C.compare y x) eqn:hc'; sis; tc; auto.
+  Defined.
+
+  Definition eq_dec :
+    forall x y : t,
+      {x = y} + {x <> y}.
+  Proof.
+    intros x y; destruct (C.compare x y) eqn:hc.
+    - left; apply C.compare_eq; auto.
+    - right; intros heq; apply C.compare_eq in heq; tc.
+    - right; intros heq; apply C.compare_eq in heq; tc.
+  Defined.
+  
+End UOT_from_UCT.
+
+Module Option_as_UOT (E : UsualOrderedType) <: UsualOrderedType.
+
+  Definition t := option E.t.
+
+  Definition eq       := @eq t.
+  Definition eq_refl  := @eq_refl t.
+  Definition eq_sym   := @eq_sym t.
+  Definition eq_trans := @eq_trans t.
+
+  Definition lt o o' :=
+    match o, o' with
+    | None, None     => False
+    | None, Some _   => True
+    | Some _, None   => False
+    | Some x, Some y => E.lt x y
+    end.
+
+  Lemma lt_trans :
+    forall x y z, lt x y -> lt y z -> lt x z.
+  Proof.
+    unfold lt; intros x y z hl hl';
+      destruct x as [x |]; destruct y as [y |]; destruct z as [z |];
+        try contradiction; auto.
+    eapply E.lt_trans; eauto.
+  Qed.
+
+  Lemma lt_not_eq :
+    forall x y,
+      lt x y -> ~ x = y.
+  Proof.
+    intros x y hl heq; destruct x as [x |]; destruct y as [y |]; tc; auto.
+    inv heq; eapply E.lt_not_eq; eauto.
+    red; auto.
+  Qed.
+
+  Definition compare :
+    forall x y,
+      Compare lt eq x y.
+  Proof.
+    intros x y; destruct x as [x |]; destruct y as [y |].
+    - destruct (E.compare x y) as [hl | he | hl].
+      + apply LT; unfold lt; auto.
+      + apply EQ; red; red in he; subst; auto.
+      + apply GT; unfold lt; auto.
+    - apply GT; red; auto.
+    - apply LT; red; auto.
+    - apply EQ; red; auto.
+  Defined.
+
+  Definition eq_dec :
+    forall x y : t,
+      {x = y} + {x <> y}.
+  Proof.
+    intros x y; destruct (compare x y) as [hl | he | hl].
+    - right; apply lt_not_eq; auto.
+    - left; subst; auto.
+    - right; intros he; subst.
+      eapply lt_not_eq; eauto.
+  Defined.
+
+End Option_as_UOT.
+
+Module List_as_UOT (E : UsualOrderedType) <: UsualOrderedType.
+
+  Definition t := list E.t.
+
+  Definition eq       := @eq t.
+  Definition eq_refl  := @eq_refl t.
+  Definition eq_sym   := @eq_sym t.
+  Definition eq_trans := @eq_trans t.
+
+  Fixpoint lt xs ys :=
+    match xs, ys with
+    | [], []             => False
+    | [], _ :: _         => True
+    | _ :: _, []         => False
+    | x :: xs', y :: ys' =>
+      match E.compare x y with
+      | LT _ => True
+      | EQ _ => lt xs' ys'
+      | GT _ => False
+      end
+    end.
+
+  Lemma lt_trans_heads_eq :
+    forall x y xs ys zs,
+      lt (x :: xs) (y :: ys)
+      -> lt (y :: ys) (x :: zs)
+      -> y = x.
+  Proof.
+    intros x y xs ys zs hl hl'; red in hl, hl'.
+    destruct (E.compare x y) as [hel | hee | hel];
+      destruct (E.compare y x) as [hel' | hee' | hel'];
+      try contradiction; auto.
+    eapply E.lt_trans in hel'; eauto.
+    exfalso; eapply E.lt_not_eq; eauto; red; auto.
+  Qed.
+
+  Lemma lt_inv_cons :
+    forall x xs ys,
+      lt (x :: xs) (x :: ys)
+      -> lt xs ys.
+  Proof.
+    intros x xs ys hl; red in hl.
+    destruct (E.compare x x); try contradiction; auto.
+    exfalso; eapply E.lt_not_eq; eauto; red; auto.
+  Qed.
+
+  Lemma lt_trans_heads_lt_or_eq :
+    forall x y z xs ys zs,
+      lt (x :: xs) (y :: ys)
+      -> lt (y :: ys) (z :: zs)
+      -> E.lt x z \/ z = x.
+  Proof.
+    intros x y z xs ys zs hl hl'; red in hl, hl'.
+    destruct (E.compare x y) as [hel | hee | hel];
+      destruct (E.compare y z) as [hel' | hee' | hel'];
+      try contradiction; auto.
+    - left; eapply E.lt_trans; eauto.
+    - left; red in hee'; subst; auto.
+    - left; red in hee ; subst; auto.
+    - right; red in hee; red in hee'; subst; auto.
+  Qed.
+  
+  Lemma lt_trans :
+    forall xs ys zs,
+      lt xs ys -> lt ys zs -> lt xs zs.
+  Proof.
+    intros xs; induction xs as [| x xs IH];
+      intros ys zs hl hl'; destruct ys as [| y ys]; destruct zs as [| z zs]; try contradiction; auto.
+    red; destruct (E.compare x z) as [hel | hee | hel]; auto.
+    - fold lt; red in hee; subst.
+      assert (heq : y = z) by (eapply lt_trans_heads_eq; eauto); subst.
+      apply lt_inv_cons in hl; apply lt_inv_cons in hl'; eauto.
+    - eapply lt_trans_heads_lt_or_eq in hl'; eauto.
+      destruct hl' as [hl' | ?]; subst.
+      + eapply E.lt_trans in hl'; eauto.
+        eapply E.lt_not_eq; eauto; red; auto.
+      + eapply E.lt_not_eq; eauto; red; auto.
+  Qed.
+  
+  Lemma lt_not_eq :
+    forall xs ys,
+      lt xs ys -> ~ xs = ys.
+  Proof.
+    intros xs; induction xs as [| x xs IH];
+      intros ys hl heq; destruct ys as [| y ys]; tc; inv heq; auto.
+    red in hl; destruct (E.compare y y); tc.
+    - eapply E.lt_not_eq; eauto; red; auto.
+    - eapply IH; eauto. 
+  Qed.
+
+  Definition compare :
+    forall xs ys,
+      Compare lt eq xs ys.
+  Proof.
+    intros xs; induction xs as [| x xs IH]; intros ys; destruct ys as [| y ys].
+    - apply EQ; red; auto.
+    - apply LT; red; auto.
+    - apply GT; red; auto.
+    - destruct (E.compare x y) as [hl | he | hl] eqn:hc.
+      + apply LT; red; rewrite hc; auto.
+      + red in he; subst.
+        destruct (IH ys) as [hl' | he' | hl'].
+        * apply LT; red; rewrite hc; auto.
+        * apply EQ; tc.
+        * apply GT; red; rewrite hc; auto.
+      + apply GT; red.
+        destruct (E.compare y x) as [hl' | he' | hl']; auto.
+        * red in he'; subst.
+          exfalso; eapply E.lt_not_eq; eauto; red; auto.
+        * eapply E.lt_trans in hl'; eauto.
+          eapply E.lt_not_eq; eauto; red; auto.
+  Defined.
+
+  Definition eq_dec :
+    forall xs ys : t,
+      {xs = ys} + {xs <> ys}.
+  Proof.
+    intros xs ys; destruct (compare xs ys) as [hl | he | hl].
+    - right; apply lt_not_eq; auto.
+    - left; subst; auto.
+    - right; intros he; subst.
+      eapply lt_not_eq; eauto.
+  Defined.
+
+End List_as_UOT.
+
+Module Nat_as_OT_Alt <: OrderedTypeAlt := OrderedType_to_Alt Nat_as_OT.
+
+(* Dumping this here for now *)
+
+
+(*
+
+
+Lemma foo :
+  forall x y,
+    compareNT x y = NO.compare (nat_of_nt x) (nat_of_nt y).
+Proof.
+  intros x y; destruct x; destruct y; auto.
+Qed.
+
+Lemma compareNT_sym :
+  forall x y,
+  compareNT y x = CompOpp (compareNT x y).
+Proof.
+  intros x y; repeat rewrite foo.
+  apply NO.compare_sym.
+Qed.
+
+Lemma compareNT_trans :
+  forall c x y z,
+    compareNT    x y = c
+    -> compareNT y z = c
+    -> compareNT x z = c.
+Proof.
+  intros c x y z hc hc'.
+  repeat rewrite foo in *.
+  eapply NO.compare_trans; eauto.
+Qed.
+
+Module NT_as_OT_Alt <: OrderedTypeAlt.
+  Definition t := nonterminal.
+  Definition compare := compareNT.
+  Definition compare_sym := compareNT_sym.
+  Definition compare_trans := compareNT_trans.
+End NT_as_OT_Alt.
+
+Module NT_as_OT <: OrderedType := OrderedType_from_Alt NT_as_OT_Alt.
+*)
+
+(*
+  Module NT_as_UOT <: UsualOrderedType.
+
+    Definition t := nonterminal.
+
+    Definition eq       := @eq nonterminal.
+    Definition eq_refl  := @eq_refl nonterminal.
+    Definition eq_sym   := @eq_sym nonterminal.
+    Definition eq_trans := @eq_trans nonterminal.
+
+    Definition lt (x y : nonterminal) : Prop :=
+      match compareNT x y with
+      | Lt => True
+      | _  => False
+      end.
+
+    Lemma lt_trans :
+      forall x y z, lt x y -> lt y z -> lt x z.
+    Proof.
+      unfold lt; intros x y z hlt hlt'.
+        destruct (compareNT x y) eqn:hb  ;
+        destruct (compareNT y z) eqn:hb' ;
+        destruct (compareNT x z) eqn:hb''; auto.
+      - eapply compareNT_trans in hb'; eauto; tc.
+      - eapply compareNT_trans in hb'; eauto; tc.
+    Qed.
+    
+    Lemma lt_not_eq :
+      forall x y, lt x y -> ~ x = y.
+    Proof.
+      unfold lt; intros x y hl heq.
+      apply compareNT_eq in heq.
+      rewrite heq in hl; inv hl.
+    Qed.
+
+    Lemma compareNT_refl :
+      forall x, compareNT x x = Eq.
+    Proof.
+      intros x; apply compareNT_eq; auto.
+    Qed.
+
+    Lemma compareNT_sym :
+      forall x y, compareNT x y = CompOpp (compareNT y x).
+    Proof.
+      intros x y; destruct (compareNT x y) eqn:hc.
+      - apply compareNT_eq in hc; subst.
+        rewrite compareNT_refl; auto.
+      - destruct (compareNT y x) eqn:hc'; auto.
+        + exfalso; apply compareNT_eq in hc'; subst.
+          rewrite compareNT_refl in hc; tc.
+        + exfalso; eapply compareNT_trans in hc'; eauto.
+          rewrite compareNT_refl in hc'; tc.
+      - destruct (compareNT y x) eqn:hc'; auto.
+        + exfalso; apply compareNT_eq in hc'; subst.
+          rewrite compareNT_refl in hc; tc.
+        + exfalso; eapply compareNT_trans in hc'; eauto.
+          rewrite compareNT_refl in hc'; tc.
+    Qed.
+
+    Definition compare :
+      forall x y,
+        Compare lt eq x y.
+    Proof.
+      intros x y; destruct (compareNT x y) eqn:hc.
+      - apply EQ; apply compareNT_eq; auto.
+      - apply LT; unfold lt; rewrite hc; auto.
+      - apply GT; unfold lt; rewrite  compareNT_sym in hc.
+        destruct (compareNT y x) eqn:hc'; sis; tc; auto.
+    Defined.
+
+    Definition eq_dec := nt_eq_dec.
+    
+  End NT_as_UOT.
+ *)
